FxyLang/Implementation/NEList.lean
@@ -4,44 +4,67 @@
   Authors: Arthur Paulino
 -/
 
-/-- Non-empty list -/
+/-
+This file contains definitions for `NEList`, an inductive type meant to
+represent non-empty lists.
+
+They are used to encode the arguments of a function or the parameters used to
+make functions applications.
+
+For example, in `f x y := ⋯ `, `x` and `y` will become members of a
+`NEList String`. And in `f (a + 2) 5`, `(a + 2)` and `5` will become members of
+a `NEList Expression`. We'll see more about those soon.
+-/
+
 inductive NEList (α : Type)
   | uno  : α → NEList α
   | cons : α → NEList α → NEList α
 
+/-- Builds an `NEList α` from a term of `α` and a term of `List α` -/
 def List.toNEList (a : α) : List α → NEList α
   | []      => .uno a
   | b :: bs => .cons a (toNEList b bs)
 
+/-- Returns `true` iff a list doesn't have duplicated elements -/
 def List.noDup [BEq α] : List α → Bool
   | []      => true
   | a :: as => ¬as.contains a && as.noDup
 
+/-- The length of a `NEList` -/
 def NEList.length : NEList α → Nat
   | uno  _   => 1
-  | cons _ l => 1 + l.length
+  | cons _ l => l.length + 1
 
+/-- Performs a fold-left on a `NEList`
+
+The `specialize` tag forces the compiler to create a version of the function
+for each `f` used for optimization purposes -/
 @[specialize]
 def NEList.foldl (f : α → β → α) : (init : α) → NEList β → α
   | a, uno  b   => f a b
   | a, cons b l => foldl f (f a b) l
 
+/-- Performs a map on a `NEList` -/
 @[specialize]
 def NEList.map (f : α → β) : NEList α → NEList β
-  | uno  a     => uno  (f a)
-  | cons a  as => cons (f a) (map f as)
+  | uno  a    => uno  (f a)
+  | cons a as => cons (f a) (map f as)
 
+/-- Builds a string with each element of a `NEList` separated by a whitespace -/
 def NEList.unfoldStrings (l : NEList String) : String :=
   l.foldl (init := "") $ fun acc a => acc ++ s!" {a}" |>.trimLeft
 
+/-- Whether an `NEList α` contains a certain term of `α` -/
 def NEList.contains [BEq α] : NEList α → α → Bool
   | uno  a,    x => a == x
   | cons a as, x => a == x || as.contains x
 
+/-- Returns `true` iff the non-empty list doesn't have duplicated elements -/
 def NEList.noDup [BEq α] : NEList α → Bool
   | uno  a    => true
   | cons a as => ¬as.contains a && as.noDup
 
+/-- Creates a term of `List α` from the elements of a term of `NEList α` -/
 def NEList.toList : NEList α → List α
   | uno  a   => [a]
   | cons a b => a :: b.toList
